Algoritmos Aproximados/Envasado.dfy/EnvasadoKAproximado.dfy
@@ -1,0 +1,7 @@
+include "../../Especificaciones/Envasado/Envasado.dfy"
+
+ghost predicate isKAproximatedBinPacking(A : multiset<nat>, E : nat, I:multiset<multiset<nat>>, k: nat)
+{
+       isEnvasado(A, E, I)
+    && forall I': multiset<multiset<nat>> | isEnvasado(A, E, I') :: |I'| * k >= |I|
+}
